tidying

src/TL.lean
@@ -26,6 +26,10 @@ inductive term : Type
 
 open term
 
+-- * * * * * * * * * * * * * * * * * * * * * * * * * * * * * * * * * * * * * * * 
+-- Notation and derived operators 
+-- * * * * * * * * * * * * * * * * * * * * * * * * * * * * * * * * * * * * * * * 
+
 notation `<0>` := var 0
 notation `<1>` := var 1
 notation `<2>` := var 2
@@ -41,61 +45,65 @@ notation `⁎` := star    -- input \asterisk
 notation `⊤` := top     --       \top
 notation `⊥` := bot     -- input \bot
 infixr ` ⟹ `:60 := imp -- input \==>
-infixr ` ∧' ` :70 := and -- input \wedge'
-infixr ` ∨' ` :59 := or  -- input \vee'
+infixr ` ⊓ ` :70 := and -- input \glb or \sqcap
+infixr ` ⊔ ` :59 := or  -- input \lub or ⊔
 
 def not (p : term) := p ⟹ ⊥
 prefix `∼`:max := not -- input \~, the ASCII character ~ has too low precedence
 
-def biimp (p q: term) := and (p ⟹ q) (q ⟹ p)
+def biimp (p q: term) := (p ⟹ q) ⊓ (q ⟹ p)
 infix ` ⇔ `:60 := biimp -- input \<=>
 
 infix ∈ := elem
 infix ∉ := λ a, λ α, not (elem a α)
-notation `⁅` φ `⁆` := comp φ
+notation `⟦` φ `⟧` := comp φ
+
+infix `××` :max := prod
 
 prefix `∀'`:1 := all 
-prefix `∃'`:2 := ex 
+prefix `∃'`:2 := ex
 
 def eq (a : term) (a' : term) : term := ∀' (a ∈ <0>) ⇔ (a' ∈ <0>)
 infix `≃` :50 := eq
 
-def singleton (a : term) := ⁅a ≃ (<0>)⁆
+def singleton (a : term) := ⟦a ≃ (<0>)⟧
 
 def ex_unique (φ : term) : term :=
-  ∃' ⁅φ⁆ ≃ singleton (<3>)
+  ∃' ⟦φ⟧ ≃ singleton (<3>)
 prefix `∃!'`:2 := ex_unique
 
 def subseteq (α : term) (β : term) : term :=
   ∀' (<0> ∈ α) ⟹ (<0> ∈ β)
 infix ⊆ := subseteq
 
+-- * * * * * * * * * * * * * * * * * * * * * * * * * * * * * * * * * * * * * * *
+
 inductive WF : context → term → type → Prop
 | star {Γ}           : WF Γ term.star 𝟙
 | top  {Γ}           : WF Γ term.top Ω
 | bot  {Γ}           : WF Γ term.bot Ω
-| and  {Γ e₁ e₂}     : WF Γ e₁ Ω → WF Γ e₁ Ω → WF Γ (term.and e₁ e₂) Ω
-| or   {Γ e₁ e₂}     : WF Γ e₁ Ω → WF Γ e₁ Ω → WF Γ (term.or e₁ e₂) Ω
-| imp  {Γ e₁ e₂}     : WF Γ e₁ Ω → WF Γ e₁ Ω → WF Γ (term.imp e₁ e₂) Ω
-| var  {Γ n A}       : list.nth Γ n = some A → WF Γ (term.var n) A
-| comp {Γ e A}       : WF (A::Γ) e Ω → WF Γ (term.comp e) (𝒫 A)
-| all  {Γ e A}       : WF (A::Γ) e Ω → WF Γ (term.all e) Ω
-| ex   {Γ e A}       : WF (A::Γ) e Ω → WF Γ (term.all e) Ω
-| elem {Γ e₁ e₂ A}   : WF Γ e₁ A → WF Γ e₂ (𝒫 A) → WF Γ (term.elem e₁ e₂) Ω
-| prod {Γ e₁ e₂ A B} : WF Γ e₁ A → WF Γ e₂ B → WF Γ (term.prod e₁ e₂) (A ×× B)
+| and  {Γ e₁ e₂}     : WF Γ e₁ Ω → WF Γ e₁ Ω → WF Γ (e₁ ⊓ e₂) Ω
+| or   {Γ e₁ e₂}     : WF Γ e₁ Ω → WF Γ e₁ Ω → WF Γ (e₁ ⊔ e₂) Ω
+| imp  {Γ e₁ e₂}     : WF Γ e₁ Ω → WF Γ e₁ Ω → WF Γ (e₁ ⟹ e₂) Ω
+| var  {Γ n A}       : list.nth Γ n = some A → WF Γ (var n) A
+| comp {Γ e A}       : WF (A::Γ) e Ω → WF Γ ⟦e⟧ (𝒫 A)
+| all  {Γ e A}       : WF (A::Γ) e Ω → WF Γ (∀' e) Ω
+| ex   {Γ e A}       : WF (A::Γ) e Ω → WF Γ (∃' e) Ω
+| elem {Γ e₁ e₂ A}   : WF Γ e₁ A → WF Γ e₂ (𝒫 A) → WF Γ (e₁ ∈ e₂) Ω
+| prod {Γ e₁ e₂ A B} : WF Γ e₁ A → WF Γ e₂ B → WF Γ (prod e₁ e₂) (A ×× B)
 
 def subst_nth (b:term) : ℕ → term → term
 | n star       := star
 | n top        := top
 | n bot        := bot
-| n (and p q)  := and (subst_nth n p) (subst_nth n q)
-| n (or p q)   := or (subst_nth n p) (subst_nth n q)
-| n (imp p q)  := imp (subst_nth n p) (subst_nth n q)
+| n (p ⊓ q)    := (subst_nth n p) ⊓ (subst_nth n q)
+| n (p ⊔ q)    := (subst_nth n p) ⊔ (subst_nth n q)
+| n (p ⟹ q)  := (subst_nth n p) ⟹ (subst_nth n q)
 | n (var m)    := if n=m then b else var m
-| n (comp φ)   := comp (subst_nth (n+1) φ)
-| n (all φ)    := all (subst_nth (n+1) φ)
-| n (ex φ)     := ex (subst_nth (n+1) φ)
-| n (elem a α) := elem (subst_nth n a) (subst_nth n α)
+| n ⟦φ⟧        := ⟦subst_nth (n+1) φ⟧
+| n (∀' φ)     := ∀' (subst_nth (n+1) φ)
+| n (∃' φ)     := ∃' (subst_nth (n+1) φ)
+| n (a ∈ α)    := (subst_nth n a) ∈ (subst_nth n α)
 | n (prod a b) := prod (subst_nth n a) (subst_nth n b)
 
 def subst (b:term):= subst_nth b 0
@@ -104,30 +112,30 @@ def remap_vars : Π k : ℕ, (ℕ → ℕ) → term → term
 | k σ top        := top
 | k σ star       := star
 | k σ bot        := bot
-| k σ (p ∧' q)   := (remap_vars k σ p) ∧' (remap_vars k σ q)
-| k σ (p ∨' q)   := (remap_vars k σ p) ∨' (remap_vars k σ q)
+| k σ (p ⊓ q)   := (remap_vars k σ p) ⊓ (remap_vars k σ q)
+| k σ (p ⊔ q)   := (remap_vars k σ p) ⊔ (remap_vars k σ q)
 | k σ (p ⟹ q)  := (remap_vars k σ p) ⟹ (remap_vars k σ q)
 | k σ (var m)    := var (σ (m+k))
-| k σ (⁅φ⁆)      := ⁅(remap_vars (k+1) σ φ)⁆
-| k σ (∀' φ)     := ∀' (remap_vars (k+1) σ φ)
-| k σ (∃' φ)     := ex (remap_vars (k+1) σ φ)
+| k σ ⟦φ⟧         := ⟦remap_vars (k+1) σ φ⟧
+| k σ (∀' φ)     := ∀' remap_vars (k+1) σ φ
+| k σ (∃' φ)     := ∃' remap_vars (k+1) σ φ
 | k σ (a ∈ α)    := (remap_vars k σ a) ∈ (remap_vars k σ α)
 | k σ (prod a b) := prod (remap_vars k σ a) (remap_vars k σ b)
 
 inductive proof : context → term → term → Prop
--- c1-3??
+-- c1-3 unecessary?? (because free variables must appear in context)
 | axm        {Γ φ}     : WF Γ φ Ω → proof Γ φ φ
 | vac        {Γ φ}     : WF Γ φ Ω → proof Γ φ term.top
 | abs        {Γ φ}     : WF Γ φ Ω → proof Γ term.bot φ
 | cut        {Γ φ ψ γ} : proof Γ φ ψ → proof Γ ψ γ → proof Γ φ γ
-| and_intro  {Γ p q r} : proof Γ p q → proof Γ p r → proof Γ p (q ∧' r)  
-| and_left   {Γ p q r} : proof Γ p (q ∧' r) → proof Γ p q
-| and_right  {Γ p q r} : proof Γ p (q ∧' r) → proof Γ p r
-| or_intro   {Γ p q r} : proof Γ p r → proof Γ q r → proof Γ (p ∨' q) r  
-| or_left    {Γ p q r} : proof Γ (p ∨' q) r → proof Γ p r
-| or_right   {Γ p q r} : proof Γ (p ∨' q) r → proof Γ q r
-| imp_to_and {Γ p q r} : proof Γ p (q ⟹ r) → proof Γ (p ∧' q) r
-| and_to_imp {Γ p q r} : proof Γ (p ∧' q) r → proof Γ p (q ⟹ r)
+| and_intro  {Γ p q r} : proof Γ p q → proof Γ p r → proof Γ p (q ⊓ r)  
+| and_left   {Γ p q r} : proof Γ p (q ⊓ r) → proof Γ p q
+| and_right  {Γ p q r} : proof Γ p (q ⊓ r) → proof Γ p r
+| or_intro   {Γ p q r} : proof Γ p r → proof Γ q r → proof Γ (p ⊔ q) r  
+| or_left    {Γ p q r} : proof Γ (p ⊔ q) r → proof Γ p r
+| or_right   {Γ p q r} : proof Γ (p ⊔ q) r → proof Γ q r
+| imp_to_and {Γ p q r} : proof Γ p (q ⟹ r) → proof Γ (p ⊓ q) r
+| and_to_imp {Γ p q r} : proof Γ (p ⊓ q) r → proof Γ p (q ⟹ r)
 
 | apply    {Γ φ ψ b B} :
     WF Γ b B
@@ -142,7 +150,7 @@ inductive proof : context → term → term → Prop
 | comp       {Γ φ A}   :
     WF (A::A::Γ) φ Ω
     → proof Γ ⊤
-      (∀' (<0> ∈ (comp φ)) ⇔ (subst <0> φ))
+      (∀' (<0> ∈ ⟦φ⟧) ⇔ (subst <0> φ))
 
 | ext                  :
     proof [] ⊤ $ 
@@ -154,11 +162,15 @@ inductive proof : context → term → term → Prop
 
 | prod_distinct_rep    :
     proof [] ⊤
-      ∀' ∀' ∀' ∀' (prod <3> <1> ≃ prod <2> <0>) ⟹ (<3> ≃ <2> ∧' <1> ≃ <0>)
+      ∀' ∀' ∀' ∀' (prod <3> <1> ≃ prod <2> <0>) ⟹ (<3> ≃ <2> ⊓ <1> ≃ <0>)
 
 example : proof [] ⊤ ⊤ := proof.axm WF.top
 
 lemma proof_WF {Γ : context} {P Q: term} : WF Γ P Ω → proof Γ P Q → WF Γ Q Ω := sorry
+
+variables p q r : term
+
+example {Γ : context}  : proof Γ ⊤ (q ⟹ r) → proof Γ q r := sorry
 
 def FV {Γ : context} {A : type} (a : term): WF Γ a A → context := λ _, Γ
 
